@prefix dcterms: <http://purl.org/dc/terms/> .
@prefix foaf: <http://xmlns.com/foaf/0.1/> .
@prefix ns1: <http://purl.obolibrary.org/obo/> .
@prefix ns2: <http://nfdi.fiz-karlsruhe.de/ontology/> .
@prefix ns3: <http://www.geneontology.org/formats/oboInOwl#> .
@prefix ns4: <https://nfdi.fiz-karlsruhe.de/ontology/> .
@prefix ns5: <http://emmo.info/emmo#> .
@prefix owl: <http://www.w3.org/2002/07/owl#> .
@prefix rdfs: <http://www.w3.org/2000/01/rdf-schema#> .
@prefix schema: <https://schema.org/> .
@prefix skos: <http://www.w3.org/2004/02/skos/core#> .
@prefix xsd: <http://www.w3.org/2001/XMLSchema#> .

ns2:Consortium a owl:Class ;
    rdfs:label "consortium"@en ;
    ns2:example "NFDI4Culture, NFDI-MatWerk, DataPLANT." ;
    rdfs:comment "NFDI consortia grouped by a discipline based in a science-led process managed by the German Research Foundation (DFG)."@en ;
    rdfs:subClassOf ns2:Organization .

ns2:DataPortal a owl:Class ;
    rdfs:label "data portal"@en ;
    ns2:example "Bach digital, KultSam, MusiXplora"@en ;
    rdfs:comment "An online platform that provides access to data collections and datasets."@en ;
    rdfs:subClassOf <http://schema.org/Service> .

ns2:ProvidedResource a owl:Class ;
    rdfs:label "provided resource"@en ;
    rdfs:comment "A ressource that identifies a resource provided to the nfdi."@en ;
    rdfs:subClassOf ns2:Resource .

ns2:Publication a owl:Class ;
    rdfs:label "publication"@en ;
    ns2:example "MusiXplora: Visual analysis of a musicological encyclopedia, Textkategorien in kompositorischen Werkstattdokumenten" ;
    rdfs:comment "A published scholarly work that reports on ongoing activity about or within a resource, e.g. a dataset."@en ;
    rdfs:subClassOf <http://schema.org/CreativeWork> .

ns2:ServiceType a owl:Class ;
    rdfs:label "service type"@en ;
    ns2:example "Expertise, advertisement, curation"@en ;
    rdfs:comment "A resource that identifies the type of a service."@en .

ns2:bestPractice a owl:ObjectProperty ;
    rdfs:label "best practice"@en ;
    rdfs:comment "The property is a relationship between a resource and the best practice."@en ;
    rdfs:domain ns2:Resource ;
    rdfs:range ns2:Specification ;
    owl:inverseOf ns2:bestPracticeOf .

ns2:country a owl:ObjectProperty ;
    rdfs:label "country"@en ;
    rdfs:comment "The property relates a city or a state to a country where it is located."@en ;
    rdfs:range ns2:Country ;
    owl:inverseOf ns2:countryOf .

ns2:federalState a owl:ObjectProperty ;
    rdfs:label "federal state"@en ;
    rdfs:comment "The property relates a city to a federal state where it is located."@en ;
    rdfs:domain ns2:City ;
    rdfs:range ns2:FederalState ;
    owl:inverseOf ns2:federalStateOf .

ns2:fundingOrganisation a owl:ObjectProperty ;
    rdfs:label "funding organisation"@en ;
    rdfs:comment "The property relates a resource or a project to the organisation that provided funding for it."@en ;
    rdfs:range ns2:Organization ;
    rdfs:subPropertyOf ns2:funder ;
    owl:inverseOf ns2:fundingOrganisationOf .

ns2:fundingProject a owl:ObjectProperty ;
    rdfs:label "funding project"@en ;
    rdfs:comment "The property relateds a resource to the project that provided funding for it."@en ;
    rdfs:domain ns2:Resource ;
    rdfs:range ns2:Project ;
    rdfs:subPropertyOf ns2:funder ;
    owl:inverseOf ns2:fundingProjectOf .

ns2:location a owl:ObjectProperty ;
    rdfs:label "location"@en ;
    rdfs:comment "The property is a relationship between a thing and a place its located at. "@en ;
    rdfs:domain owl:Thing ;
    rdfs:range ns2:Place ;
    owl:inverseOf ns2:locationOf .

ns2:objectType a owl:ObjectProperty ;
    rdfs:label "object type"@en ;
    rdfs:comment "The property relates a data collection to the type of object it contains. "@en ;
    rdfs:domain ns2:Collection ;
    rdfs:range ns2:ObjectType ;
    owl:inverseOf ns2:objectTypeOf .

ns2:parentOrganisation a owl:ObjectProperty ;
    rdfs:label "parent organisation"@en ;
    rdfs:comment "The property is a parental relationship between organisations."@en ;
    rdfs:domain ns2:Organization ;
    rdfs:range ns2:Organization ;
    owl:inverseOf ns2:subsidiaryOrganization .

ns2:partnerOrganization a owl:ObjectProperty,
        owl:SymmetricProperty ;
    rdfs:domain ns2:Organization ;
    rdfs:range ns2:Organization .

ns2:programmingLanguage a owl:ObjectProperty ;
    rdfs:label "programming language"@en ;
    rdfs:comment "The property links software to a programming language it is written in." ;
    rdfs:domain ns2:Software ;
    rdfs:range ns2:ProgrammingLanguage ;
    owl:inverseOf ns2:programmingLanguageOf .

ns2:publisher a owl:ObjectProperty ;
    rdfs:label "publisher"@en ;
    rdfs:comment "The property is a relationship between a resource and an organisation or a person responsible for publishing it."@en ;
    rdfs:domain ns2:Resource ;
    owl:inverseOf ns2:publisherOf .

ns2:relatedProject a owl:ObjectProperty,
        owl:SymmetricProperty ;
    rdfs:label "related project"@en ;
    rdfs:comment "The property is a relationship between related projects. The property is symmetric."@en ;
    rdfs:domain ns2:Project ;
    rdfs:range ns2:Project .

ns2:semanticExpressivity a owl:ObjectProperty ;
    rdfs:label "semantic expressivity"@en ;
    rdfs:comment "The property relates a resource to its semantic expressivity spectrum."@en ;
    rdfs:domain <http://purls.helmholtz-metadaten.de/mwo/SemanticResource> ;
    rdfs:range ns2:SemanticExpressivity ;
    owl:inverseOf ns2:semanticExpressivityOf .

ns2:standard a owl:ObjectProperty ;
    rdfs:label "standard"@en ;
    rdfs:comment "The property relates a resource to the standard it relies on."@en ;
    rdfs:domain ns2:Resource ;
    rdfs:range ns2:Standard ;
    owl:inverseOf ns2:standardOf .

dcterms:isPartOf a owl:ObjectProperty ;
    rdfs:domain ns2:TaskArea ;
    rdfs:range ns4:Consortium .

dcterms:title a owl:AnnotationProperty,
        owl:DatatypeProperty ;
    rdfs:label "has title"@en ;
    rdfs:comment "A name given to a resource.  Typically, the title will be the name by which the resource is formally known."@en ;
    rdfs:domain ns2:Resource .

<http://purls.helmholtz-metadaten.de/mwo/ChemistryDatabase> a owl:Class ;
    rdfs:label "chemistry database"@en ;
    ns1:IAO_0000115 "A database containing chemistry data."@en ;
    rdfs:subClassOf <http://purls.helmholtz-metadaten.de/mwo/Database> .

<http://purls.helmholtz-metadaten.de/mwo/ComputationalWorkflow> a owl:Class ;
    rdfs:label "computational workflow"@en ;
    ns1:IAO_0000115 "A computational workflow is a workflow which describes the complex multi-step methods that are used for data collection, data preparation, analytics, predictive modelling, and simulation that lead to new data products."@en ;
    ns3:hasDbXref <https://doi.org/10.1162/dint_a_00033> ;
    rdfs:subClassOf <http://purls.helmholtz-metadaten.de/mwo/Workflow>,
        <http://www.ebi.ac.uk/swo/SWO_0000001> .

<http://purls.helmholtz-metadaten.de/mwo/ContactPerson> a owl:Class ;
    rdfs:label "contact person"@en ;
    ns1:IAO_0000115 "A role which inheres in a bearer and is realised when this person acts as the contact point regarding a contribution."@en ;
    rdfs:subClassOf ns1:BFO_0000023,
        <http://purls.helmholtz-metadaten.de/mwo/ContactPoint> .

<http://purls.helmholtz-metadaten.de/mwo/CrystallographyDatabase> a owl:Class ;
    rdfs:label "crystallography database"@en ;
    ns1:IAO_0000115 "A database containing crystal structures and data on structural and mathematical crystallography, solid state physics and structural chemistry."@en ;
    rdfs:subClassOf <http://purls.helmholtz-metadaten.de/mwo/Database> .

<http://purls.helmholtz-metadaten.de/mwo/DataCollector> a owl:Class ;
    rdfs:label "data collector"@en ;
    ns1:IAO_0000115 "A role which inheres in a bearer and is realised when this bearer has participated in the gathering of data."@en ;
    rdfs:comment "The bearer in this definition might be a person or a software agent. Data may consist of subject data, object data or both."@en ;
    rdfs:subClassOf ns1:BFO_0000023 .

<http://purls.helmholtz-metadaten.de/mwo/EducationalResource> a owl:Class ;
    rdfs:label "educational resource"@en ;
    ns1:IAO_0000115 "A resource or material that can be used for teaching and learning puposes."@en ;
    rdfs:subClassOf ns2:Resource .

<http://purls.helmholtz-metadaten.de/mwo/ElectronicLabNotebook> a owl:Class ;
    rdfs:label "electronic lab notebook"@en ;
    ns1:IAO_0000115 "An Electronic Lab Notebook is a software tool that digitally replicates paper lab notebooks traditionally used in the sciences to record experimental results. It allows scientists to access, search, and share results from an experiment."@en ;
    ns3:hasExactSynonym "Electronic Laboratory Notebook"@en ;
    rdfs:subClassOf <http://www.ebi.ac.uk/swo/SWO_0000001> .

<http://purls.helmholtz-metadaten.de/mwo/ExperimentalWorkflow> a owl:Class ;
    rdfs:label "Experimental Workflow"@en ;
    ns1:IAO_0000115 "Experimental workflow is a workflow that describes an experimental process, including the design, preparation, measurement, and analysis of the data."@en ;
    rdfs:subClassOf <http://purls.helmholtz-metadaten.de/mwo/Workflow> .

<http://purls.helmholtz-metadaten.de/mwo/GitRepository> a owl:Class ;
    rdfs:label "git repository" ;
    ns1:IAO_0000115 "A repository that is created and managed using a Git version control system."@en ;
    rdfs:subClassOf <http://purls.helmholtz-metadaten.de/mwo/Repository> .

<http://purls.helmholtz-metadaten.de/mwo/LargeScaleFacility> a owl:Class ;
    rdfs:label "large-scale facility"@en ;
    ns1:IAO_0000115 "A facility that provides access to large-scale scientific equipment and allows scientists to carry out state-of-the-art research."@en .

<http://purls.helmholtz-metadaten.de/mwo/Lecture> a owl:Class ;
    rdfs:label "Lecture" ;
    ns1:IAO_0000115 "An academic event which is intented to deliver instruction on a specific topic, most commonly to an audience of university students."@en ;
    rdfs:subClassOf <http://purls.helmholtz-metadaten.de/mwo/EducationalEvent> .

<http://purls.helmholtz-metadaten.de/mwo/MaterialsDatabase> a owl:Class ;
    rdfs:label "materials database"@en ;
    ns1:IAO_0000115 "A database containing data of experimental and computational properties of materials"@en ;
    rdfs:subClassOf <http://purls.helmholtz-metadaten.de/mwo/Database> .

<http://purls.helmholtz-metadaten.de/mwo/MetadataSchema> a owl:Class ;
    rdfs:label "metadata schema"@en ;
    ns1:IAO_0000115 "A metadata schema is a specification which establishes the elements needed to describe a data resource in a formalized and concise manner."@en ;
    rdfs:subClassOf ns2:Specification .

<http://purls.helmholtz-metadaten.de/mwo/OntologyRepository> a owl:Class ;
    rdfs:label "ontology repository"@en ;
    ns1:IAO_0000115 "A repository which contains ontologies."@en ;
    rdfs:subClassOf <http://purls.helmholtz-metadaten.de/mwo/Repository> .

<http://purls.helmholtz-metadaten.de/mwo/Patent> a owl:Class ;
    rdfs:label "patent"@en ;
    ns1:IAO_0000115 "A patent is an exclusive right granted for an invention, which is a product or a process that provides, in general, a new way of doing something, or offers a new technical solution to a problem. To get a patent, technical information about the invention must be disclosed to the public in a patent application."@en ;
    ns3:hasDbXref <https://www.wipo.int/patents/en/> ;
    rdfs:subClassOf ns2:Specification .

<http://purls.helmholtz-metadaten.de/mwo/PotentialsRepository> a owl:Class ;
    rdfs:label "potentials repository"@en ;
    ns1:IAO_0000115 "A data repository which contains interatomic potentials or pseudopotentials for atomistic models."@en ;
    rdfs:subClassOf <http://purls.helmholtz-metadaten.de/mwo/Repository> .

<http://purls.helmholtz-metadaten.de/mwo/ProcessingSoftware> a owl:Class ;
    rdfs:label "processing software"@en ;
    ns1:IAO_0000115 "Software which carries out a (planned) process on digital data,"@en ;
    rdfs:comment "Depending on the temporal relation of the carried out process to an analysis process, the process might either be termed \"pre-processing\" (e.g. converting file formats) or \"post-processing\" (e.g. spatial filtering of images)."@en ;
    rdfs:subClassOf <http://www.ebi.ac.uk/swo/SWO_0000001> .

<http://purls.helmholtz-metadaten.de/mwo/ProjectLeader> a owl:Class ;
    rdfs:label "project leader"@en ;
    ns1:IAO_0000115 "A role which inheres in a bearer and is realized when an person is responsible for 1) the coordination of project resources and 2) the operations carried out within it."@en ;
    ns3:hasDbXref <https://www.indeed.com/career-advice/finding-a-job/project-leader-vs-project-manager> ;
    ns3:hasRelatedSynonym <http://purls.helmholtz-metadaten.de/mwo/ProjectManager> ;
    rdfs:comment "In a project, a project leader might engage, motivate and support the team by establishing and maintaining productive operations"@en ;
    rdfs:subClassOf ns1:BFO_0000023 .

<http://purls.helmholtz-metadaten.de/mwo/ResearchSoftware> a owl:Class ;
    rdfs:label "research software"@en ;
    ns1:IAO_0000115 "Software which was created for a research purpose."@en ;
    ns3:hasDbXref <https://doi.org/10.5281/zenodo.5504016> ;
    ns3:hasExactSynonym "Scientific software"@en ;
    rdfs:comment """Software components (e.g., operating systems, libraries, dependencies, packages, scripts, etc.) that are used for research but were not created during or with a clear research intent should be considered software in research and not Research Software. This differentiation may vary between disciplines.
Research software might be source code files, algorithms, scripts, computational workflows and executables"""@en ;
    rdfs:subClassOf <http://www.ebi.ac.uk/swo/SWO_0000001> .

<http://purls.helmholtz-metadaten.de/mwo/Seminar> a owl:Class ;
    rdfs:label "Seminar"@en ;
    ns1:IAO_0000115 "An academic event where recuring meetings are held on a particular research topic, usually attended by academic and research staff."@en ;
    rdfs:subClassOf <https://w3id.org/scholarlydata/ontology/conference-ontology.owl#AcademicEvent> .

<http://purls.helmholtz-metadaten.de/mwo/SoftwareRepository> a owl:Class ;
    rdfs:label "software repository"@en ;
    ns1:IAO_0000115 "A repository which contains software and its components, including libraries, scripts, etc."@en ;
    rdfs:subClassOf <http://purls.helmholtz-metadaten.de/mwo/Repository> .

<http://purls.helmholtz-metadaten.de/mwo/SummerSchool> a owl:Class ;
    rdfs:label "Summer School"@en ;
    ns1:IAO_0000115 "An academic event where a school session is conducted in summer enabling students to accelerate progress toward a diploma or degree, to make up credits lost through absence or failure, or to round out professional education."@en ;
    ns3:hasDbXref <https://www.merriam-webster.com/dictionary/summer%20school#:~:text=noun,to%20round%20out%20professional%20education> ;
    rdfs:subClassOf <http://purls.helmholtz-metadaten.de/mwo/EducationalEvent> .

<http://purls.helmholtz-metadaten.de/mwo/TrainingCourse> a owl:Class ;
    rdfs:label "Training Course"@en ;
    ns1:IAO_0000115 "An academic event where the objective is to teach skills needed for a particular task or job."@en ;
    rdfs:subClassOf <http://purls.helmholtz-metadaten.de/mwo/EducationalEvent> .

<http://purls.helmholtz-metadaten.de/mwo/VisualizationSoftware> a owl:Class ;
    rdfs:label "visualization software"@en ;
    ns1:IAO_0000115 "Software which creates graphical representations of data, features of data or data sets."@en ;
    ns3:hasBroadSynonym "Graphics software"@en ;
    rdfs:subClassOf <http://www.ebi.ac.uk/swo/SWO_0000001> .

<http://purls.helmholtz-metadaten.de/mwo/WorkflowEnvironment> a owl:Class ;
    rdfs:label "workflow environment"@en ;
    ns1:IAO_0000115 "A workflow environment is a software that manages and allows the user to create and interact with computational workflows."@en ;
    rdfs:subClassOf <http://www.ebi.ac.uk/swo/SWO_0000001> .

<http://purls.helmholtz-metadaten.de/mwo/aboutMaterial> a owl:ObjectProperty ;
    rdfs:label "about material"@en ;
    ns1:IAO_0000115 "A relation between a dataset and the material it contains data on."@en ;
    rdfs:domain ns2:Dataset ;
    rdfs:range ns5:EMMO_4207e895_8b83_4318_996a_72cfb32acd94 .

<http://purls.helmholtz-metadaten.de/mwo/belongsTo> a owl:ObjectProperty ;
    rdfs:label "belongs to"@en ;
    ns1:IAO_0000115 "A relation between a research group or large-scale facility and the organization it belongs to."@en ;
    rdfs:range ns2:Organization .

<http://purls.helmholtz-metadaten.de/mwo/conformsToSpecification> a owl:ObjectProperty ;
    rdfs:label "conforms to specification"@en ;
    ns1:IAO_0000115 "A relation between a resource and the specification it conforms to."@en ;
    rdfs:domain ns2:Resource ;
    rdfs:range ns2:Specification .

<http://purls.helmholtz-metadaten.de/mwo/description> a owl:DatatypeProperty ;
    rdfs:label "description"@en ;
    ns1:IAO_0000115 "A data property linking an entity to its description."@en .

<http://purls.helmholtz-metadaten.de/mwo/emailAddress> a owl:DatatypeProperty ;
    rdfs:label "email address"@en .

<http://purls.helmholtz-metadaten.de/mwo/hasAcronym> a owl:DatatypeProperty ;
    rdfs:label "has acronym"@en ;
    ns1:IAO_0000115 "A data property indicating the acronym of an entity, often represented as an abbreviation of the initials of the name or title of the entity."@en .

<http://purls.helmholtz-metadaten.de/mwo/hasAffiliation> a owl:ObjectProperty ;
    rdfs:label "has affiliation"@en ;
    ns1:IAO_0000115 "a relation between a person and an organization to which the person is affiliated."@en ;
    rdfs:domain ns2:Person ;
    rdfs:range ns2:Organization .

<http://purls.helmholtz-metadaten.de/mwo/hasContactPoint> a owl:ObjectProperty ;
    rdfs:label "a relation between a thing and its contact point, which can be a person or website."@en,
        "has contact point"@en ;
    rdfs:domain owl:Thing ;
    rdfs:range <http://purls.helmholtz-metadaten.de/mwo/ContactPoint> .

<http://purls.helmholtz-metadaten.de/mwo/hasContributor> a owl:ObjectProperty ;
    rdfs:label "has contributor"@en ;
    owl:inverseOf <http://purls.helmholtz-metadaten.de/mwo/isContributorOf> .

<http://purls.helmholtz-metadaten.de/mwo/hasCreator> a owl:ObjectProperty ;
    rdfs:label "has creator" ;
    ns1:IAO_0000115 "A relation between a dataset and a person or organization, who has created the data."@en ;
    rdfs:domain ns2:Dataset ;
    rdfs:subPropertyOf <http://purls.helmholtz-metadaten.de/mwo/hasAuthor> .

<http://purls.helmholtz-metadaten.de/mwo/hasDOI> a owl:DatatypeProperty ;
    rdfs:label "has DOI" ;
    ns1:IAO_0000115 "A data property relating a work to its Digital Object Identifier (DOI)."@en ;
    rdfs:domain ns2:Resource ;
    rdfs:subPropertyOf dcterms:identifier .

<http://purls.helmholtz-metadaten.de/mwo/hasDiscipline> a owl:ObjectProperty ;
    rdfs:label "has discipline"@en ;
    ns1:IAO_0000115 "A relation between a resource or large-scale facility and the academic discipline of the produced work."@en ;
    rdfs:domain ns2:Resource ;
    rdfs:range ns2:AcademicDiscipline .

<http://purls.helmholtz-metadaten.de/mwo/hasDocumentation> a owl:ObjectProperty ;
    rdfs:label "has documentation"@en ;
    ns1:IAO_0000115 "A relation between a resource and its documentation."@en ;
    rdfs:domain ns2:Resource ;
    rdfs:range <http://purls.helmholtz-metadaten.de/mwo/Documentation> .

<http://purls.helmholtz-metadaten.de/mwo/hasEndpointURL> a owl:DatatypeProperty ;
    rdfs:label "has endpoint URL"@en ;
    ns1:IAO_0000115 "A data property relating a SPARQL EndPoint with its URL."@en ;
    rdfs:domain <http://purls.helmholtz-metadaten.de/mwo/SparqlEndpoint> ;
    rdfs:range xsd:anyURI ;
    rdfs:subPropertyOf ns2:url .

<http://purls.helmholtz-metadaten.de/mwo/hasExpertiseIn> a owl:ObjectProperty ;
    rdfs:label "has expertise in"@en ;
    ns1:IAO_0000115 "A relation between a person and an academic discipline or research topic, in which this person is an expert."@en ;
    rdfs:domain ns2:Person ;
    rdfs:range ns2:AcademicDiscipline .

<http://purls.helmholtz-metadaten.de/mwo/hasFormat> a owl:ObjectProperty ;
    rdfs:label "has format"@en ;
    ns1:IAO_0000115 "The file format of the resource"@en ;
    rdfs:domain ns2:Resource ;
    rdfs:range dcterms:FileFormat .

<http://purls.helmholtz-metadaten.de/mwo/hasLeader> a owl:ObjectProperty ;
    rdfs:label "has leader"@en ;
    ns1:IAO_0000115 "A relation between a research group and its leader."@en ;
    rdfs:domain <http://purls.helmholtz-metadaten.de/mwo/ResearchGroup> ;
    rdfs:range <http://purls.helmholtz-metadaten.de/mwo/GroupLeader> ;
    owl:inverseOf <http://purls.helmholtz-metadaten.de/mwo/isLeaderOf> .

<http://purls.helmholtz-metadaten.de/mwo/hasLecturer> a owl:ObjectProperty ;
    rdfs:label "has lecturer"@en ;
    ns1:IAO_0000115 "A relation between an academic event and a person, who participates in teaching capacity in the event."@en ;
    rdfs:range ns2:Person .

<http://purls.helmholtz-metadaten.de/mwo/hasManual> a owl:ObjectProperty ;
    rdfs:label "has manual"@en ;
    ns1:IAO_0000115 "A relation between an instrument and its documentation."@en ;
    rdfs:domain <https://w3id.org/skgo/modsci#Instrument> ;
    rdfs:range <http://purls.helmholtz-metadaten.de/mwo/Documentation> .

<http://purls.helmholtz-metadaten.de/mwo/hasMember> a owl:ObjectProperty ;
    rdfs:label "has member"@en ;
    ns1:IAO_0000115 "A relation between a research project and its members."@en ;
    rdfs:domain ns2:Project ;
    rdfs:range <http://purls.helmholtz-metadaten.de/mwo/ProjectMember> ;
    owl:inverseOf <http://purls.helmholtz-metadaten.de/mwo/memberOf> .

<http://purls.helmholtz-metadaten.de/mwo/hasORCID> a owl:DatatypeProperty ;
    rdfs:label "has ORCID" ;
    ns1:IAO_0000115 "A data property relating a person to their Open Researcher and Contributor ID (ORCID)." ;
    rdfs:domain ns2:Person ;
    rdfs:subPropertyOf dcterms:identifier .

<http://purls.helmholtz-metadaten.de/mwo/hasOwner> a owl:ObjectProperty ;
    rdfs:label "has owner"@en ;
    ns1:IAO_0000115 "A relation between an instrument and the organization that acts as its owner."@en ;
    rdfs:domain <https://w3id.org/skgo/modsci#Instrument> ;
    rdfs:range ns2:Organization .

<http://purls.helmholtz-metadaten.de/mwo/hasPostalCode> a owl:DatatypeProperty ;
    rdfs:label "has postal code" ;
    ns1:IAO_0000115 "A data property indicating the postal code of an entity." ;
    rdfs:subPropertyOf <http://purls.helmholtz-metadaten.de/mwo/hasPostalAddress> .

<http://purls.helmholtz-metadaten.de/mwo/hasProjectIdentifier> a owl:DatatypeProperty ;
    rdfs:label "has project identifier"@en ;
    ns1:IAO_0000115 "A data property relating a research project with a unique identifier, defined in a given context."@en ;
    rdfs:domain ns2:Project ;
    rdfs:subPropertyOf dcterms:identifier .

<http://purls.helmholtz-metadaten.de/mwo/hasRORID> a owl:DatatypeProperty ;
    rdfs:label "has ROR ID" ;
    ns1:IAO_0000115 "A data property relating an organization to its identifier within the Research Organization Registry (ROR)."@en ;
    rdfs:domain ns2:Organization ;
    rdfs:subPropertyOf dcterms:identifier .

<http://purls.helmholtz-metadaten.de/mwo/hasRelatedResource> a owl:ObjectProperty,
        owl:SymmetricProperty ;
    rdfs:label "has related resource"@en ;
    ns1:IAO_0000115 "A relation between two different resources, which indicates both are associated."@en ;
    rdfs:domain ns2:Resource ;
    rdfs:range ns2:Resource .

<http://purls.helmholtz-metadaten.de/mwo/hasRepository> a owl:ObjectProperty ;
    rdfs:label "has repository"@en ;
    ns1:IAO_0000115 "A relation between a software and the website of the repository where it is stored."@en ;
    rdfs:domain ns2:Resource ;
    rdfs:range <http://purls.helmholtz-metadaten.de/mwo/Repository> .

<http://purls.helmholtz-metadaten.de/mwo/hasRole> a owl:ObjectProperty ;
    rdfs:label "has role"@en ;
    ns1:IAO_0000115 "A relation between a person (the bearer) and a role, in which the role specifically depends on the bearer for its existence."@en ;
    rdfs:domain ns2:Person ;
    rdfs:range ns1:BFO_0000023 .

<http://purls.helmholtz-metadaten.de/mwo/hasSerialNumber> a owl:DatatypeProperty ;
    rdfs:label "has serial number"@en ;
    rdfs:comment "A data property linking something, for example a piece of equipment, to its serial number."@en ;
    rdfs:subPropertyOf dcterms:identifier .

<http://purls.helmholtz-metadaten.de/mwo/hasSparqlEndpoint> a owl:ObjectProperty ;
    rdfs:label "has SPARQL endpoint"@en ;
    ns1:IAO_0000115 "A relation between a semantic resource and its SPARQL Endpoint."@en ;
    rdfs:domain <http://purls.helmholtz-metadaten.de/mwo/SemanticResource> ;
    rdfs:range <http://purls.helmholtz-metadaten.de/mwo/SparqlEndpoint> .

<http://purls.helmholtz-metadaten.de/mwo/hasTopic> a owl:ObjectProperty ;
    rdfs:label "has topic"@en ;
    ns1:IAO_0000115 "A relation between a research project and the topic of the research question it investigates."@en ;
    rdfs:domain ns2:Project ;
    rdfs:range <http://purls.helmholtz-metadaten.de/mwo/ResearchTopic> .

<http://purls.helmholtz-metadaten.de/mwo/hasVersion> a owl:DatatypeProperty ;
    rdfs:label "has version"@en ;
    ns1:IAO_0000115 "A number or string that identifies different variants or releases of a resource."@en ;
    rdfs:domain ns2:Resource .

<http://purls.helmholtz-metadaten.de/mwo/hasWebsite> a owl:ObjectProperty ;
    rdfs:label "has website"@en ;
    ns1:IAO_0000115 "a relation between a thing and its website."@en ;
    rdfs:domain owl:Thing ;
    rdfs:range ns2:Website .

<http://purls.helmholtz-metadaten.de/mwo/instrumentModel> a owl:DatatypeProperty ;
    rdfs:label "instrument model"@en ;
    ns1:IAO_0000115 "A data property relating an instrument with the model information."@en ;
    rdfs:domain <https://w3id.org/skgo/modsci#Instrument> .

<http://purls.helmholtz-metadaten.de/mwo/isOnline> a owl:DatatypeProperty ;
    rdfs:label "is online"@en ;
    ns1:IAO_0000115 "A flag to indicate an organized event or educational resource can be accessed online."@en ;
    rdfs:range xsd:boolean .

<http://purls.helmholtz-metadaten.de/mwo/keyword> a owl:DatatypeProperty ;
    rdfs:label "keywords"@en ;
    ns1:IAO_0000115 "A data property used for defining something with keywords."@en .

<http://purls.helmholtz-metadaten.de/mwo/mainTaskArea> a owl:ObjectProperty ;
    rdfs:domain <http://purls.helmholtz-metadaten.de/mwo/UseCase> ;
    rdfs:range ns2:TaskArea .

<http://purls.helmholtz-metadaten.de/mwo/relatedParticipantProject> a owl:ObjectProperty ;
    rdfs:domain <http://purls.helmholtz-metadaten.de/mwo/UseCase> ;
    rdfs:range <http://purls.helmholtz-metadaten.de/mwo/ParticipantProject> .

<http://purls.helmholtz-metadaten.de/mwo/relatedTaskArea> a owl:ObjectProperty ;
    rdfs:domain <http://purls.helmholtz-metadaten.de/mwo/UseCase> ;
    rdfs:range ns2:TaskArea .

<http://purls.helmholtz-metadaten.de/mwo/requiredTool> a owl:ObjectProperty ;
    rdfs:label "required tool"@en ;
    ns1:IAO_0000115 "A relation between an educational resource or academic event and the tools required to participate."@en ;
    rdfs:range <http://www.ebi.ac.uk/swo/SWO_0000001> .

<http://purls.helmholtz-metadaten.de/mwo/softwareCitation> a owl:ObjectProperty ;
    rdfs:label "software citation"@en ;
    ns1:IAO_0000115 "A relation between a work and a cited software."@en ;
    rdfs:domain ns2:Resource ;
    rdfs:range ns2:Software ;
    rdfs:subPropertyOf schema:citation .

<http://purls.helmholtz-metadaten.de/mwo/usesMethod> a owl:ObjectProperty ;
    rdfs:label "uses method"@en ;
    ns1:IAO_0000115 "A relation between a resource and method it implements, uses or describes."@en ;
    rdfs:domain ns2:Resource ;
    rdfs:range <http://purls.helmholtz-metadaten.de/mwo/Method> .

<http://purls.helmholtz-metadaten.de/mwo/usesTechnology> a owl:ObjectProperty ;
    rdfs:label "uses technology"@en ;
    ns1:IAO_0000115 "A relation between an instrument and the technology it implements."@en ;
    rdfs:domain <https://w3id.org/skgo/modsci#Instrument> ;
    rdfs:range <https://w3id.org/skgo/modsci#Technology> .

<http://purls.helmholtz-metadaten.de/mwo/workingOnTopic> a owl:ObjectProperty ;
    rdfs:label "a relation between a research group and the topic in which it conducts research."@en,
        "working on topic"@en ;
    rdfs:domain <http://purls.helmholtz-metadaten.de/mwo/ResearchGroup> ;
    rdfs:range <http://purls.helmholtz-metadaten.de/mwo/ResearchTopic> .

<http://www.ebi.ac.uk/swo/SWO_0000020> a owl:Class ;
    rdfs:label "Unix" ;
    rdfs:subClassOf <http://www.ebi.ac.uk/swo/SWO_0000021> .

<http://www.ebi.ac.uk/swo/SWO_0000022> a owl:Class ;
    rdfs:label "Linux" ;
    rdfs:subClassOf <http://www.ebi.ac.uk/swo/SWO_0000021> .

<http://www.ebi.ac.uk/swo/SWO_0000082> a owl:ObjectProperty ;
    rdfs:label "uses software"@en ;
    ns1:IAO_0000112 "Cytoscape plugins would be linked to the Cytoscape application via uses software, while Microsoft Excel is linked to Microsoft Office via has_part." ;
    ns1:IAO_0000115 "This property allows the linkage of two different pieces of software such that one directly executes or uses the other. The has_part relationship should instead be used to describe related but independent members of a larger software package, and 'uses platform' relationship should be used to describe which operating system(s) a particular piece of software can use." ;
    ns1:IAO_0000119 "Allyson Lister" ;
    rdfs:domain <http://www.ebi.ac.uk/swo/SWO_0000001> ;
    rdfs:range <http://www.ebi.ac.uk/swo/SWO_0000001> ;
    owl:inverseOf <http://www.ebi.ac.uk/swo/SWO_0000157> .

<http://www.ebi.ac.uk/swo/SWO_0000149> a owl:Class ;
    rdfs:label "Mac OS"@en ;
    ns1:IAO_0000115 "Mac OS is software which is used as the operating system for the Macintosh personal computer created by Apple Inc." ;
    ns1:IAO_0000119 "http://en.wikipedia.org/wiki/History_of_Mac_OS, accessed 25 March 2015." ;
    dcterms:creator "Allyson Lister" ;
    rdfs:subClassOf <http://www.ebi.ac.uk/swo/SWO_0000021> .

<http://www.ebi.ac.uk/swo/SWO_0004001> a owl:ObjectProperty ;
    rdfs:label "has interface" ;
    ns1:IAO_0000115 "Provides a method of asserting what type of interactions are possible for the class in question. The interface must be from the 'software interface' hierarchy." ;
    ns1:IAO_0000119 "Allyson Lister",
        "Andy Brown" ;
    dcterms:creator "Andy Brown" ;
    rdfs:range <http://www.ebi.ac.uk/swo/SWO_9000050> .

<http://www.ebi.ac.uk/swo/SWO_9000072> a owl:Class ;
    rdfs:label "Microsoft Windows" ;
    rdfs:comment "The Windows Operating System" ;
    rdfs:subClassOf <http://www.ebi.ac.uk/swo/SWO_0000021> .

<http://www.ebi.ac.uk/swo/has_license> a owl:ObjectProperty ;
    rdfs:label "has license" ;
    ns1:IAO_0000115 "The relationship between an entity and the set of legal restrictions, i.e. license, which are applied in using or otherwise interacting with that entity. Eg. relationship between software and a software license." ;
    rdfs:domain ns2:Resource ;
    rdfs:range <http://www.ebi.ac.uk/swo/SWO_0000002> ;
    owl:inverseOf <http://www.ebi.ac.uk/swo/is_license_for> .

<http://www.ebi.ac.uk/swo/interface/SWO_9000054> a owl:Class ;
    rdfs:label "application programming interface" ;
    ns1:IAO_0000115 "An application programming interface is a set of routines, protocols, and tools for building software applications. An API expresses a software component in terms of its operations, inputs, outputs, and underlying types. An API defines functionalities that are independent of their respective implementations, which allows definitions and implementations to vary without compromising each other. The API specifies how software components should interact." ;
    ns1:IAO_0000118 "API" ;
    ns1:IAO_0000119 "http://en.wikipedia.org/wiki/Application_programming_interface, accessed 25 November 2014." ;
    rdfs:subClassOf <http://www.ebi.ac.uk/swo/SWO_9000050> .

<http://www.ebi.ac.uk/swo/license/SWO_1000001> a owl:Class ;
    rdfs:label "Creative Commons" ;
    ns1:IAO_0000118 "CC" ;
    rdfs:subClassOf <http://www.ebi.ac.uk/swo/SWO_0000002> .

<http://www.ebi.ac.uk/swo/license/SWO_1000002> a owl:Class ;
    rdfs:label "Proprietary commercial software license" ;
    rdfs:subClassOf <http://www.ebi.ac.uk/swo/SWO_0000002> .

<http://www.ebi.ac.uk/swo/license/SWO_1000009> a owl:Class ;
    rdfs:label "License without restrictions on derivatives" ;
    rdfs:subClassOf <http://www.ebi.ac.uk/swo/SWO_0000002> .

<http://www.ebi.ac.uk/swo/license/SWO_1000043> a owl:Class ;
    rdfs:label "GNU Project Free License Type" ;
    ns1:IAO_0000115 """A licensed is a free license according to GNU if the users have the four essential freedoms:

    The freedom to run the program, for any purpose (freedom 0).
    The freedom to study how the program works, and change it so it does your computing as you wish (freedom 1). Access to the source code is a precondition for this.
    The freedom to redistribute copies so you can help your neighbor (freedom 2).
    The freedom to distribute copies of your modified versions to others (freedom 3). By doing this you can give the whole community a chance to benefit from your changes. Access to the source code is a precondition for this.

A program is free software if users have all of these freedoms. Thus, you should be free to redistribute copies, either with or without modifications, either gratis or charging a fee for distribution, to anyone anywhere. Being free to do these things means (among other things) that you do not have to ask or pay for permission to do so.

“Free software” does not mean “noncommercial”. A free program must be available for commercial use, commercial development, and commercial distribution. Commercial development of free software is no longer unusual; such free commercial software is very important. You may have paid money to get copies of free software, or you may have obtained copies at no charge. But regardless of how you got your copies, you always have the freedom to copy and change the software, even to sell copies. """ ;
    ns1:IAO_0000119 "http://www.gnu.org/philosophy/free-sw.html, accessed 12 June 2013." ;
    dcterms:creator "Allyson Lister" ;
    rdfs:comment "Allyson Lister: This class defines those licenses which are free licenses, but which may or may not be compatible with any version of the GNU GPL." ;
    rdfs:subClassOf <http://www.ebi.ac.uk/swo/license/SWO_1000008> .

<http://www.ebi.ac.uk/swo/license/SWO_1000048> a owl:ObjectProperty,
        owl:SymmetricProperty ;
    rdfs:label "is compatible license of"@en ;
    ns1:IAO_0000115 "'is compatible license of' provides a method of marking two software licenses as compatible and without conflicts, e.g. that the Apache License version 2 is compatible with GNU GPL version 3. If two licenses are connected with this property, it means code released under one license can be released with code from the other license in a larger program." ;
    ns1:IAO_0000119 "http://www.gnu.org/licenses/gpl-faq.html#WhatDoesCompatMean, accessed 12 June 2013." ;
    dcterms:creator "Allyson Lister" ;
    rdfs:domain <http://www.ebi.ac.uk/swo/SWO_0000002> ;
    rdfs:range <http://www.ebi.ac.uk/swo/SWO_0000002> .

<http://www.ebi.ac.uk/swo/license/SWO_1000056> a owl:Class ;
    rdfs:label "Artistic License" ;
    dcterms:creator "Allyson Lister" ;
    rdfs:subClassOf <http://www.ebi.ac.uk/swo/SWO_0000002> .

<http://www.ebi.ac.uk/swo/license/SWO_1000061> a owl:Class ;
    rdfs:label "free to use license"@en ;
    ns1:IAO_0000115 "A license which allows any form of usage of the artifact." ;
    rdfs:subClassOf <http://www.ebi.ac.uk/swo/SWO_0000002> .

<http://www.ebi.ac.uk/swo/license/SWO_1000069> a owl:Class ;
    rdfs:label "GNU AGPL"@en ;
    rdfs:subClassOf <http://www.ebi.ac.uk/swo/SWO_0000002> .

<http://www.ebi.ac.uk/swo/license/SWO_1000095> a owl:Class ;
    rdfs:label "Open Data Commons"@en ;
    rdfs:subClassOf <http://www.ebi.ac.uk/swo/SWO_0000002> .

<http://www.ebi.ac.uk/swo/license/SWO_1000103> a owl:Class ;
    rdfs:label "Vendor-specific License"@en ;
    ns1:IAO_0000115 "A vendor-specific license is a license which was, at least originally, created by a specific organization to be used just on the resources created within that organization. This is a hierarchy of convenience rather than of shared philosophy. Many of the licenses have since been taken up by other groups whose licensing requirements matched those of the originating organization." ;
    ns1:IAO_0000119 "Allyson Lister" ;
    dcterms:creator "Allyson Lister" ;
    rdfs:subClassOf <http://www.ebi.ac.uk/swo/SWO_0000002> .

<http://www.ebi.ac.uk/swo/license/SWO_1000137> a owl:Class ;
    rdfs:label "Fee-Based Commercial License"@en ;
    ns1:IAO_0000115 "Fee-Based Commercial License is a license which, among its license clauses, states that commercial entities may use the resource for a fee." ;
    ns1:IAO_0000119 "Allyson Lister" ;
    dcterms:creator "Allyson Lister" ;
    rdfs:comment "Allyson Lister: This is a convenience class which combines multiple license clauses to create a defined class, such that any license type which meets the requirements will be inferred to fall into this category." ;
    rdfs:subClassOf <http://www.ebi.ac.uk/swo/SWO_0000002> .

<http://www.ebi.ac.uk/swo/license/SWO_1000140> a owl:Class ;
    rdfs:label "Non-Commercial No-Fee License"@en ;
    ns1:IAO_0000115 "Non-Commercial No-Fee License is a license which, among its license clauses, states that non-commercial entities may use the resource without a purchase or usage cost." ;
    ns1:IAO_0000119 "Allyson Lister" ;
    dcterms:creator "Allyson Lister" ;
    rdfs:comment "Allyson Lister: This is a convenience class which combines multiple license clauses to create a defined class, such that any license type which meets the requirements will be inferred to fall into this category." ;
    rdfs:subClassOf <http://www.ebi.ac.uk/swo/SWO_0000002> .

owl:Nothing a owl:Class ;
    rdfs:label "Nothing" ;
    owl:complementOf owl:Thing .

foaf:firstName a owl:DatatypeProperty ;
    rdfs:domain ns2:Person ;
    rdfs:subPropertyOf <http://purls.helmholtz-metadaten.de/mwo/hasPersonalInformation> .

foaf:gender a owl:DatatypeProperty,
        owl:FunctionalProperty ;
    rdfs:label "gender" ;
    rdfs:comment "The gender of this Agent (typically but not necessarily 'male' or 'female')." ;
    rdfs:domain ns2:Person ;
    rdfs:isDefinedBy foaf: ;
    rdfs:subPropertyOf <http://purls.helmholtz-metadaten.de/mwo/hasPersonalInformation> .

foaf:surname a owl:DatatypeProperty ;
    rdfs:domain ns2:Person ;
    rdfs:subPropertyOf <http://purls.helmholtz-metadaten.de/mwo/hasPersonalInformation> .

foaf:title a owl:DatatypeProperty ;
    rdfs:label "title" ;
    rdfs:comment "Title (Mr, Mrs, Ms, Dr. etc)" ;
    rdfs:domain ns2:Person ;
    rdfs:isDefinedBy foaf: ;
    rdfs:subPropertyOf <http://purls.helmholtz-metadaten.de/mwo/hasPersonalInformation> .

ns4:Person a owl:Class ;
    rdfs:label "person"@en ;
    rdfs:comment "A resource that represents a single person."@en ;
    ns4:example "Harald Sack, Tabea Tietz, Sasha Bruns, Etienne Posthumus" .

ns4:areaCode a owl:DatatypeProperty ;
    rdfs:label "area code"@en ;
    rdfs:domain ns4:Organization ;
    rdfs:range rdfs:Literal .

ns4:emailAddress a owl:DatatypeProperty ;
    rdfs:label "email address"@en ;
    rdfs:range rdfs:Literal .

ns4:fileExtension a owl:DatatypeProperty ;
    rdfs:label "file extension" ;
    rdfs:comment "An identifier for a file format (e.g. txt for a text file) used as a suffix to the file name, don't use dot at start."@en ;
    ns4:example "mp4",
        "ttl",
        "txt",
        "xml" .

ns4:fundingOrganization a owl:ObjectProperty ;
    rdfs:label "funding organization"@en ;
    rdfs:comment "The property relates a resource or a project to the organization that provided funding for it."@en ;
    rdfs:range ns4:Organization ;
    owl:inverseOf ns4:fundingOrganizationOf .

ns4:fundingProject a owl:ObjectProperty ;
    rdfs:label "funding project"@en ;
    rdfs:comment "The property relateds a resource to the project that provided funding for it."@en ;
    rdfs:range ns4:Project ;
    owl:inverseOf ns4:fundingProjectOf .

ns4:parentOrganization a owl:ObjectProperty ;
    rdfs:label "parent organization"@en ;
    rdfs:comment "The property is a parental relationship between organizations."@en ;
    rdfs:domain ns4:Organization ;
    rdfs:range ns4:Organization .

ns4:partnerOrganization a owl:ObjectProperty,
        owl:SymmetricProperty ;
    rdfs:label "partner organization"@en ;
    rdfs:comment "The property is a partner relationship between organizations. The property is symmetric."@en ;
    rdfs:domain ns4:Organization ;
    rdfs:range ns4:Organization .

ns4:relatedProject a owl:ObjectProperty ;
    rdfs:label "related project"@en ;
    rdfs:comment "The property is a relationship between a project or a resource and related projects."@en ;
    rdfs:range ns4:Project .

ns4:url a owl:DatatypeProperty ;
    rdfs:label "url"@en ;
    rdfs:comment "URL of a thing"@en ;
    rdfs:domain owl:Thing ;
    rdfs:range xsd:anyURI .

<https://w3id.org/scholarlydata/ontology/conference-ontology.owl#Conference> a owl:Class ;
    rdfs:label "Conference"@en ;
    rdfs:comment "A conference event."@en ;
    rdfs:subClassOf <https://w3id.org/scholarlydata/ontology/conference-ontology.owl#AcademicEvent> .

<https://w3id.org/scholarlydata/ontology/conference-ontology.owl#Talk> a owl:Class ;
    rdfs:label "Talk"@en ;
    rdfs:comment "A talk event."@en ;
    rdfs:subClassOf <https://w3id.org/scholarlydata/ontology/conference-ontology.owl#AcademicEvent> .

<https://w3id.org/scholarlydata/ontology/conference-ontology.owl#Tutorial> a owl:Class ;
    rdfs:label "Tutorial"@en ;
    rdfs:comment "An event which a teaching session is given to to an individual or very small group."@en ;
    rdfs:subClassOf <http://purls.helmholtz-metadaten.de/mwo/EducationalEvent> .

<https://w3id.org/scholarlydata/ontology/conference-ontology.owl#Workshop> a owl:Class ;
    rdfs:label "Workshop"@en ;
    rdfs:comment "An event which is a long interactive meeting or educational session designed to create a specialized result. Workshops are smaller than conferences, and are usually only a day or two long and are dedicated to discussing a specific topic."@en ;
    rdfs:subClassOf <https://w3id.org/scholarlydata/ontology/conference-ontology.owl#AcademicEvent> .

<https://w3id.org/scholarlydata/ontology/conference-ontology.owl#duration> a owl:DatatypeProperty ;
    rdfs:label "duration"@en ;
    rdfs:comment "duration"@en ;
    rdfs:domain <https://w3id.org/scholarlydata/ontology/conference-ontology.owl#OrganisedEvent> .

<https://w3id.org/scholarlydata/ontology/conference-ontology.owl#endDate> a owl:DatatypeProperty ;
    rdfs:label "end date"@en ;
    rdfs:comment "end date"@en ;
    rdfs:domain <https://w3id.org/scholarlydata/ontology/conference-ontology.owl#OrganisedEvent> .

<https://w3id.org/scholarlydata/ontology/conference-ontology.owl#hasSubEvent> a owl:ObjectProperty ;
    rdfs:label "has sub event"@en ;
    rdfs:comment "has sub event"@en ;
    rdfs:domain <https://w3id.org/scholarlydata/ontology/conference-ontology.owl#OrganisedEvent> ;
    rdfs:range <https://w3id.org/scholarlydata/ontology/conference-ontology.owl#OrganisedEvent> ;
    rdfs:subPropertyOf <https://w3id.org/scholarlydata/ontology/conference-ontology.owl#hasPart> ;
    owl:inverseOf <https://w3id.org/scholarlydata/ontology/conference-ontology.owl#isSubEventOf> .

<https://w3id.org/scholarlydata/ontology/conference-ontology.owl#startDate> a owl:DatatypeProperty ;
    rdfs:label "start date"@en ;
    rdfs:comment "start date"@en ;
    rdfs:domain <https://w3id.org/scholarlydata/ontology/conference-ontology.owl#OrganisedEvent> .

<https://w3id.org/seo#KeynoteSpeaker> a owl:Class ;
    rdfs:label "Keynote speaker"@en ;
    rdfs:comment "Someone who gives the main address at a formal gathering such as a conference ."@en ;
    rdfs:subClassOf <https://w3id.org/seo#InvitedSpeakers> .

<https://w3id.org/skgo/modsci#LaboratoryInstrument> a owl:Class ;
    rdfs:label "Laboratory Instrument"@en ;
    rdfs:comment "An instrument needed for operations in various laboratories, synthesis and analysis."@en ;
    rdfs:subClassOf <https://w3id.org/skgo/modsci#Instrument> ;
    owl:equivalentClass <https://w3id.org/skgo/modsci#ScientificInstrument> .

<https://w3id.org/skgo/modsci#hasManufacturer> a owl:ObjectProperty ;
    rdfs:label "has manufacturer"@en ;
    ns1:IAO_0000115 "A relation between company that makes goods for sale."@en ;
    rdfs:domain <https://w3id.org/skgo/modsci#ScientificInstrument> ;
    rdfs:range <https://w3id.org/skgo/modsci#ScientificInstrumentManufacturer> ;
    owl:inverseOf <https://w3id.org/skgo/modsci#isManufacturerOf> .

ns5:EMMO_4207e895_8b83_4318_996a_72cfb32acd94 a owl:Class ;
    rdfs:label "Material" ;
    ns5:EMMO_967080e5_2f42_4eb2_a3a9_c58143e835f9 "A matter individual that stands for a real world object representing an amount of a physical substance (or mixture of substances) in different states of matter or phases."@en ;
    rdfs:comment "An instance of a material (e.g. nitrogen) can represent different states of matter. The fact that the individual also belongs to other classes (e.g. Gas) would reveal the actual form in which the material is found."@en,
        "Material usually means some definite kind, quality, or quantity of matter, especially as intended for use."@en ;
    skos:prefLabel "Material"@en .

ns2:City a owl:Class ;
    rdfs:label "city"@en ;
    ns2:example "Berlin, Hannover, Kyiv"@en ;
    rdfs:comment "A city or a town where the thing is located."@en ;
    rdfs:subClassOf ns2:Place .

ns2:Collection a owl:Class ;
    rdfs:label "collection"@en ;
    ns2:example "RISM catalogue of musical sources"@en ;
    rdfs:comment "A tangible collection of valuables published or curated by an organisation or a person."@en ;
    rdfs:subClassOf <http://schema.org/Product> .

ns2:Country a owl:Class ;
    rdfs:label "country"@en ;
    rdfs:comment "A country where the thing is located."@en ;
    rdfs:subClassOf ns2:Place .

ns2:FederalState a owl:Class ;
    rdfs:label "federal state"@en ;
    ns2:example "Sachsen, Berlin"@de ;
    rdfs:comment "A federal state where the thing is located."@en ;
    rdfs:subClassOf ns2:Place .

ns2:ObjectType a owl:Class ;
    rdfs:label "object type"@en ;
    ns2:example "book, photograph, music sheet"@en ;
    rdfs:comment "A resource that identifies the type of object in a data collection."@en .

ns2:ProgrammingLanguage a owl:Class ;
    rdfs:label "programming language"@en ;
    ns2:example "Java, Ruby, C++, Perl, PHP" ;
    rdfs:comment "A formal language used for implementing a software."@en ;
    rdfs:subClassOf ns2:TechnologicalMeans ;
    owl:equivalentClass <https://w3id.org/skgo/modsci#ProgrammingLanguage> .

ns2:SemanticExpressivity a owl:Class ;
    rdfs:label "semantic expressivity"@en ;
    ns2:example "controlled vocabulary, ontology, taxonomy"@en ;
    rdfs:comment "An entity that identifies the level of the semantic expressivity of a resource. Five instances are now included in nfdicore."@en .

ns2:Standard a owl:Class ;
    rdfs:label "standard"@en ;
    ns2:example "ISO 15511, DINI-Zertifikat" ;
    rdfs:comment "An international standard and norm that can be used to evaluate or create services."@en ;
    rdfs:subClassOf ns2:Specification .

ns2:TechnologicalMeans a owl:Class ;
    rdfs:label "technological means"@en ;
    ns2:example "Groovy on Grails, Angular"@en ;
    rdfs:comment "A technology, e.g. a web application or a programming framework used in a resource."@en .

ns2:Website a owl:Class ;
    rdfs:label "website"@en ;
    ns2:example "https:\\/\\/opac.rism.info" ;
    rdfs:comment "A collection of webpages contributed by an organisation or a person."@en ;
    rdfs:subClassOf <http://schema.org/Product> .

ns2:bestPracticeOf a owl:ObjectProperty ;
    rdfs:label "best practice of"@en .

ns2:countryOf a owl:ObjectProperty ;
    rdfs:label "country of"@en .

ns2:federalStateOf a owl:ObjectProperty ;
    rdfs:label "federal state of"@en .

ns2:fundingOrganisationOf a owl:ObjectProperty ;
    rdfs:label "funding organisation of"@en ;
    rdfs:subPropertyOf ns2:funderOf .

ns2:fundingProjectOf a owl:ObjectProperty ;
    rdfs:label "funding project of"@en ;
    rdfs:subPropertyOf ns2:funderOf .

ns2:locationOf a owl:ObjectProperty ;
    rdfs:label "location of"@en .

ns2:objectTypeOf a owl:ObjectProperty ;
    rdfs:label "object type of"@en .

ns2:programmingLanguageOf a owl:ObjectProperty ;
    rdfs:label "programming language of"@en .

ns2:publisherOf a owl:ObjectProperty ;
    rdfs:label "publisher of"@en .

ns2:semanticExpressivityOf a owl:ObjectProperty ;
    rdfs:label "semantic expressivity of"@en .

ns2:standardOf a owl:ObjectProperty ;
    rdfs:label "standard of"@en .

ns2:subsidiaryOrganization a owl:ObjectProperty ;
    rdfs:label "subsidiary organization"@en .

ns2:url a owl:DatatypeProperty ;
    rdfs:label "url"@en ;
    rdfs:comment "URL of a thing."@en ;
    rdfs:domain owl:Thing ;
    rdfs:range xsd:anyURI .

dcterms:FileFormat a owl:Class ;
    rdfs:label "File Format"@en-us ;
    rdfs:comment "Examples include the formats defined by the list of Internet Media Types."@en-us ;
    rdfs:subClassOf dcterms:MediaType ;
    skos:definition "A digital resource format."@en-us .

dcterms:MediaType a owl:Class ;
    rdfs:label "Media Type"@en-us ;
    skos:definition "A file format or physical medium."@en-us .

<http://purls.helmholtz-metadaten.de/mwo/GroupLeader> a owl:Class ;
    rdfs:label "group leader"@en ;
    ns1:IAO_0000115 "A role which inheres in a bearer and is realized when this person holds the responsibility for the operations of a group of agents."@en ;
    ns3:hasRelatedSynonym <http://purls.helmholtz-metadaten.de/mwo/Supervisor> ;
    rdfs:comment "The responsibilities of a group leader might include, among others, guiding, motivating, supporting and coordinating the group in different scopes (i.e. scientific, administrative, financial). In scientific projects (i.e. within the NFDI context) the group in this definition will be a research group, institute or department. In most cases the group leader is also the supervisor to the group"@en ;
    rdfs:subClassOf ns1:BFO_0000023 .

<http://purls.helmholtz-metadaten.de/mwo/Method> a owl:Class ;
    rdfs:label "method"@en ;
    ns1:IAO_0000115 "A method is a systematic procedure, technique, or mode of inquiry employed by or proper to a particular discipline or art."@en ;
    ns3:hasDbXref <https://www.merriam-webster.com/dictionary/method#:~:text=a(1),the%20lecture%20method> ;
    ns3:hasExactSynonym "Approach"@en,
        "Procedure"@en,
        "Technique"@en .

<http://purls.helmholtz-metadaten.de/mwo/ParticipantProject> a owl:Class ;
    rdfs:subClassOf ns4:Project .

<http://purls.helmholtz-metadaten.de/mwo/ProjectManager> a owl:Class ;
    rdfs:label "project manager"@en ;
    ns1:IAO_0000115 "A role which inheres in a bearer and is realized when that person is responsible for 1) helping to define the project scope, goals and deliverables, 2) taking care of the budget, documentation and staffing, 3) reporting and documenting the progress, and 4) managing a project and meeting deadlines."@en ;
    ns3:hasDbXref <https://www.indeed.com/career-advice/finding-a-job/project-leader-vs-project-manager> ;
    rdfs:subClassOf ns1:BFO_0000023 .

<http://purls.helmholtz-metadaten.de/mwo/ProjectMember> a owl:Class ;
    rdfs:label "project member"@en ;
    ns1:IAO_0000115 "A role which inheres in a bearer and is realized when this bearer participates in the planning, operation or dissemination of a project."@en ;
    rdfs:subClassOf ns1:BFO_0000023 .

<http://purls.helmholtz-metadaten.de/mwo/Supervisor> a owl:Class ;
    rdfs:label "supervisor"@en ;
    ns1:IAO_0000115 "A role which inheres in a bearer and is realized when a person is responsible for 1) the coordination  and 2) the operations of another person, group or department."@en ;
    rdfs:comment "In a project with more than one member, the project leader might engage, motivate and support the team by establishing and maintaining productive operations. Note that a project leader is not necessarily the group leader."@en ;
    rdfs:subClassOf ns1:BFO_0000023 .

<http://purls.helmholtz-metadaten.de/mwo/WebService> a owl:Class ;
    rdfs:label "web service"@en ;
    ns1:IAO_0000115 "A service that supports interoperable machine-to-machine interaction over a network."@en ;
    rdfs:subClassOf <http://schema.org/Service> ;
    owl:equivalentClass <http://www.ebi.ac.uk/swo/interface/SWO_9000051> .

<http://purls.helmholtz-metadaten.de/mwo/hasAuthor> a owl:ObjectProperty ;
    rdfs:label "has author"@en ;
    ns1:IAO_0000115 "A relation between a resource and a person, who is the author."@en ;
    rdfs:domain ns2:Resource ;
    rdfs:range ns2:Person .

<http://purls.helmholtz-metadaten.de/mwo/hasPostalAddress> a owl:DatatypeProperty ;
    rdfs:label "has postal address"@en ;
    ns1:IAO_0000115 "A data property indicating the postal address of an entity."@en .

<http://purls.helmholtz-metadaten.de/mwo/isContributorOf> a owl:ObjectProperty ;
    rdfs:label "is contributor of"@en ;
    ns1:IAO_0000115 "A relation between an organization or person and the resource of which it is a contributor."@en ;
    rdfs:range ns2:Resource .

<http://purls.helmholtz-metadaten.de/mwo/isLeaderOf> a owl:ObjectProperty ;
    rdfs:label "is leader of"@en .

<http://purls.helmholtz-metadaten.de/mwo/memberOf> a owl:ObjectProperty ;
    rdfs:label "member of"@en .

<http://schema.org/Organization> a owl:Class ;
    rdfs:label "Organization"@en ;
    rdfs:comment "An organization such as a school, NGO, corporation, club, etc."@en .

<http://schema.org/Person> a owl:Class .

<http://schema.org/Project> a owl:Class ;
    rdfs:label "Project"@en ;
    rdfs:comment "An enterprise (potentially individual but typically collaborative), planned to achieve a particular aim. Use properties from Organization, subOrganization/parentOrganization to indicate project sub-structures."@en .

<http://www.ebi.ac.uk/swo/SWO_0000157> a owl:ObjectProperty ;
    rdfs:label "is software for"@en ;
    rdfs:domain <http://www.ebi.ac.uk/swo/SWO_0000001> ;
    rdfs:range <http://www.ebi.ac.uk/swo/SWO_0000001> .

<http://www.ebi.ac.uk/swo/interface/SWO_9000051> a owl:Class ;
    rdfs:label "web service" ;
    ns1:IAO_0000115 "A web service is a software interface which works as a method of communication between two electronic devices over the World Wide Web and which is provided at a particular network address. There are two major classes of Web services: REST-compliant Web services, and arbitrary (or application-specific) Web services." ;
    ns1:IAO_0000118 "Web Service" ;
    ns1:IAO_0000119 "Modified from http://www.w3.org/TR/ws-arch/, accessed 6 June 2013; Modified from http://en.wikipedia.org/wiki/Web_service, accessed 6 June 2013." ;
    dcterms:creator "Allyson Lister" ;
    rdfs:subClassOf <http://www.ebi.ac.uk/swo/SWO_9000050> .

<http://www.ebi.ac.uk/swo/is_license_for> a owl:ObjectProperty ;
    rdfs:label "is license for"@en ;
    ns1:IAO_0000115 "The relationship between an entity and the set of legal restrictions, i.e. license, which are applied in using or otherwise interacting with that entity. Eg. relationship between a software license and the software which implements it." .

<http://www.ebi.ac.uk/swo/license/SWO_1000008> a owl:Class ;
    rdfs:label "Open source software license" ;
    rdfs:subClassOf <http://www.ebi.ac.uk/swo/SWO_0000002> .

ns4:Consortium a owl:Class ;
    rdfs:label "consortium"@en ;
    rdfs:comment "NFDI consortia grouped by a discipline based in a science-led process managed by the German Research Foundation (DFG)."@en ;
    rdfs:subClassOf ns4:Organization ;
    ns4:example "NFDI4Culture, NFDI-MatWerk, DataPLANT." .

ns4:fundingOrganizationOf a owl:ObjectProperty ;
    rdfs:label "funding organization of"@en .

ns4:fundingProjectOf a owl:ObjectProperty ;
    rdfs:label "funding project of"@en .

schema:dateCreated a owl:DatatypeProperty ;
    rdfs:label "dateCreated"@en ;
    rdfs:comment "The date on which the CreativeWork was created or the item was added to a DataFeed."@en ;
    rdfs:domain ns2:Resource ;
    rdfs:isDefinedBy schema:dateCreated .

schema:datePublished a owl:DatatypeProperty ;
    rdfs:label "datePublished"@en ;
    rdfs:comment "Date of first broadcast/publication."@en ;
    rdfs:domain ns2:Resource ;
    rdfs:isDefinedBy schema:datePublished .

schema:free a owl:DatatypeProperty ;
    rdfs:label "free"@en ;
    rdfs:comment "A flag to signal that the item, event, or place is accessible for free."@en ;
    rdfs:isDefinedBy schema:free .

schema:operatingSystem a owl:ObjectProperty ;
    rdfs:label "operatingSystem"@en ;
    rdfs:comment "Operating systems supported (Windows 7, OS X 10.6, Android 1.6)."@en ;
    rdfs:domain ns2:Software ;
    rdfs:isDefinedBy schema:operatingSystem ;
    rdfs:range <http://www.ebi.ac.uk/swo/SWO_0000021> .

schema:sponsor a owl:ObjectProperty ;
    rdfs:label "sponsor"@en ;
    rdfs:comment "A person or organization that supports a thing through a pledge, promise, or financial contribution. E.g. a sponsor of a Medical Study or a corporate sponsor of an event."@en ;
    rdfs:domain <https://w3id.org/scholarlydata/ontology/conference-ontology.owl#OrganisedEvent> ;
    rdfs:isDefinedBy schema:sponsor .

<https://w3id.org/scholarlydata/ontology/conference-ontology.owl#hasPart> a owl:ObjectProperty ;
    rdfs:label "has part"@en ;
    rdfs:comment "has part"@en ;
    rdfs:domain owl:Thing ;
    rdfs:range owl:Thing ;
    owl:inverseOf <https://w3id.org/scholarlydata/ontology/conference-ontology.owl#isPartOf> .

<https://w3id.org/scholarlydata/ontology/conference-ontology.owl#isSubEventOf> a owl:ObjectProperty ;
    rdfs:label "is sub event of"@en ;
    rdfs:comment "is sub event of"@en ;
    rdfs:subPropertyOf <https://w3id.org/scholarlydata/ontology/conference-ontology.owl#isPartOf> .

<https://w3id.org/seo#InvitedSpeakers> a owl:Class ;
    rdfs:label "Invited speakers"@en ;
    rdfs:comment "Invited person to give a speech in an event."@en ;
    rdfs:subClassOf ns2:Person .

<https://w3id.org/skgo/modsci#ModernScience> a owl:Class ;
    rdfs:label "Science" ;
    rdfs:comment "Science is a systematic enterprise that builds and organizes knowledge in the form of testable explanations and predictions about the universe." .

<https://w3id.org/skgo/modsci#ProgrammingLanguage> a owl:Class ;
    rdfs:label "Programming Language" ;
    rdfs:comment "A programming language is a formal language, which comprises a set of instructions that produce various kinds of output. Programming languages are used in computer programming to implement algorithms." ;
    rdfs:subClassOf <http://schema.org/ComputerLanguage> .

<https://w3id.org/skgo/modsci#ScientificInstrumentManufacturer> a owl:Class ;
    rdfs:label "Scientific Instrument Manufacturer" ;
    rdfs:comment "Companies manufacturing equipment for scientific sstudies." .

<https://w3id.org/skgo/modsci#Technology> a owl:Class ;
    rdfs:label "Technology" ;
    rdfs:comment "Technology is the collection of techniques, skills, methods, and processes used in the production of goods or services or in the accomplishment of objectives, such as scientific investigation." .

<https://w3id.org/skgo/modsci#isManufacturerOf> a owl:ObjectProperty ;
    rdfs:label "is manufacturer of"@en .

ns2:Dataset a owl:Class ;
    rdfs:label "dataset"@en ;
    rdfs:comment "A dataset is associated with a structured information about a resource."@en ;
    rdfs:subClassOf <http://schema.org/CreativeWork> .

ns2:funder a owl:ObjectProperty ;
    rdfs:label "funder"@en ;
    rdfs:comment "The property relates a thing to an organisation or a project that provided funding for it. The sub-properties are used to specify more specific funding relationships. "@en ;
    rdfs:domain owl:Thing ;
    owl:inverseOf ns2:funderOf .

<http://purls.helmholtz-metadaten.de/mwo/ContactPoint> a owl:Class ;
    rdfs:label "contact point"@en ;
    ns1:IAO_0000115 "A contact point is a person, website or e-mail which provides information concerning a resource."@en ;
    ns3:hasExactSynonym "Point of contact"@en .

<http://purls.helmholtz-metadaten.de/mwo/Documentation> a owl:Class ;
    rdfs:label "documentation"@en ;
    ns1:IAO_0000115 "Documentation is any communicable material that is used to describe, explain or instruct regarding some attributes of an object, system or procedure, such as its parts, assembly, installation, maintenance and use"@en ;
    rdfs:subClassOf <http://schema.org/Product> .

<http://purls.helmholtz-metadaten.de/mwo/ResearchGroup> a owl:Class ;
    rdfs:label "research group"@en ;
    ns1:IAO_0000115 "A group of people who work in a university or research institute and carry research on one or more topics."@en .

<http://purls.helmholtz-metadaten.de/mwo/ResearchTopic> a owl:Class ;
    rdfs:label "research topic"@en ;
    ns1:IAO_0000115 "A research topic is a specific field of study within a broader academic discipline."@en ;
    ns3:hasBroadSynonym "Research area"@en ;
    ns3:hasExactSynonym "Research field"@en,
        "Research subject"@en ;
    rdfs:subClassOf ns2:AcademicDiscipline .

<http://purls.helmholtz-metadaten.de/mwo/SemanticResource> a owl:Class ;
    rdfs:label "semantic resource" ;
    ns1:IAO_0000115 "A machine-actionable controlled vocabularies to describe the meaning of the content and express relations among them."@en ;
    rdfs:subClassOf ns2:Resource .

<http://purls.helmholtz-metadaten.de/mwo/SparqlEndpoint> a owl:Class ;
    rdfs:label "SPARQL endpoint"@en ;
    ns1:IAO_0000115 "A SPARQL endpoint is a web service that provides an access point for receiving and processing SPARQL protocol requests"@en ;
    rdfs:subClassOf <http://purls.helmholtz-metadaten.de/mwo/WebService> .

<http://purls.helmholtz-metadaten.de/mwo/Workflow> a owl:Class ;
    rdfs:label "workflow"@en ;
    ns1:IAO_0000115 "A workflow is a specification which describes a repeatable sequence of steps needed to create or produce a work."@en ;
    rdfs:subClassOf ns2:Specification .

<http://schema.org/ComputerLanguage> a owl:Class ;
    rdfs:label "ComputerLanguage"@en ;
    rdfs:comment "This type covers computer programming languages such as Scheme and Lisp, as well as other language-like computer representations. Natural languages are best represented with the <a class=\"localLink\" href=\"https://schema.org/Language\">Language</a> type."@en ;
    rdfs:isDefinedBy <http://schema.org/ComputerLanguage> ;
    rdfs:subClassOf <http://schema.org/Intangible> .

<http://schema.org/CreativeWork> a owl:Class .

<http://schema.org/Intangible> a owl:Class .

schema:citation a owl:ObjectProperty ;
    rdfs:label "citation"@en ;
    rdfs:comment "A citation or reference to another creative work, such as another publication, web page, scholarly article, etc."@en ;
    rdfs:domain ns2:Resource ;
    rdfs:isDefinedBy schema:citation ;
    rdfs:range ns2:Resource .

<https://w3id.org/scholarlydata/ontology/conference-ontology.owl#isPartOf> a owl:ObjectProperty ;
    rdfs:label "is part of"@en ;
    rdfs:comment "is part of"@en .

<https://w3id.org/skgo/modsci#ScientificInstrument> a owl:Class ;
    rdfs:label "Scientific Instrument" ;
    rdfs:comment "A scientific instrument is, broadly speaking, a device or tool used for scientific purposes, including the study of both natural phenomena and theoretical research."@en ;
    rdfs:subClassOf <https://w3id.org/skgo/modsci#Instrument> ;
    skos:prefLabel "Instrument"@en .

ns2:AcademicDiscipline a owl:Class ;
    rdfs:label "academic discipline"@en ;
    ns2:example <https://www.wikidata.org/entity/Q12271>,
        "Architecture, Art History, Musicology, Media Studies, Performing Arts"@en ;
    rdfs:comment "An academic discipline, a research field or domain of a resource, e.g. a data portal or a field of study of a person."@en ;
    rdfs:subClassOf <https://w3id.org/skgo/modsci#ModernScience> .

ns2:Software a owl:Class ;
    rdfs:label "software"@en ;
    ns2:example "Edirom, Muscat" ;
    rdfs:comment "A computer software provided by an organisation or a person."@en ;
    rdfs:subClassOf <http://schema.org/Product> ;
    owl:equivalentClass <http://www.ebi.ac.uk/swo/SWO_0000001> .

ns2:TaskArea a owl:Class .

ns2:funderOf a owl:ObjectProperty ;
    rdfs:label "funder of"@en .

<http://purls.helmholtz-metadaten.de/mwo/Database> a owl:Class ;
    rdfs:label "database"@en ;
    rdfs:comment "A structured collection of logically related data usually stored and retrieved using computer-based means."@en ;
    rdfs:subClassOf <http://schema.org/Product> .

<http://purls.helmholtz-metadaten.de/mwo/UseCase> a owl:Class .

<http://schema.org/Service> a owl:Class ;
    rdfs:label "Service"@en ;
    rdfs:comment "A service provided by an organization, e.g. delivery service, print services, etc."@en ;
    rdfs:isDefinedBy <http://schema.org/Service> ;
    rdfs:subClassOf <http://schema.org/Intangible> .

<http://www.ebi.ac.uk/swo/SWO_9000050> a owl:Class ;
    rdfs:label "software interface" ;
    ns1:IAO_0000115 "The mode of interaction with a piece of software." .

ns4:Project a owl:Class ;
    rdfs:label "project"@en ;
    rdfs:comment "A scientific or business endeavor that aims to conclude an investigation or to answer a research question."@en ;
    ns4:example "Freischütz digital, Corpus Vitrearum Medii Aevi" .

ns2:Place a owl:Class ;
    rdfs:label "place"@en ;
    ns2:example "Hessen, Berlin, Schweiz" ;
    rdfs:comment "A spatial region, e.g. country, city or district."@en .

<http://purls.helmholtz-metadaten.de/mwo/EducationalEvent> a owl:Class ;
    rdfs:label "educational event" ;
    ns1:IAO_0000115 "An organized event with the purpose of teaching knowledge to others by displaying educational materials."@en ;
    rdfs:subClassOf <https://w3id.org/scholarlydata/ontology/conference-ontology.owl#OrganisedEvent> .

<http://purls.helmholtz-metadaten.de/mwo/hasPersonalInformation> a owl:DatatypeProperty ;
    rdfs:label "has personal information"@en ;
    ns1:IAO_0000115 "A data property linking a person with information about that person."@en ;
    rdfs:domain ns2:Person .

<https://w3id.org/scholarlydata/ontology/conference-ontology.owl#AcademicEvent> a owl:Class ;
    rdfs:label "Academic event"@en ;
    rdfs:comment "Academic events are e.g. conferences and conference-like events, and all the sub-events of those which are about the topic or theme of the conference, such as talks or panels."@en ;
    rdfs:subClassOf <https://w3id.org/scholarlydata/ontology/conference-ontology.owl#OrganisedEvent> .

<http://purls.helmholtz-metadaten.de/mwo/Repository> a owl:Class ;
    rdfs:label "repository"@en ;
    rdfs:comment "A central location in which data is stored and managed."@en ;
    rdfs:subClassOf <http://schema.org/Product> .

<http://www.ebi.ac.uk/swo/SWO_0000021> a owl:Class ;
    rdfs:label "operating system" ;
    ns1:IAO_0000115 "An operating system is a piece of software which is responsible for managing software that runs on a computer and the interactions of that software with the hardware and system resources." ;
    rdfs:subClassOf <http://www.ebi.ac.uk/swo/SWO_0000001> .

ns2:Project a owl:Class ;
    rdfs:label "project"@en ;
    ns2:example "Freisch\\u00fctz digital, Corpus Vitrearum Medii Aevi" ;
    rdfs:comment "A scientific or business endeavour that aims to conclude an investigation or to answer a research question."@en ;
    owl:equivalentClass <http://schema.org/Project> .

ns2:Specification a owl:Class ;
    rdfs:label "specification"@en ;
    ns2:example "RDF, SPARQL, Federation" ;
    rdfs:comment "A set of requirements, guidelines, standards contributed by an organisation or a person."@en ;
    rdfs:subClassOf <http://schema.org/Product> .

<https://w3id.org/skgo/modsci#Instrument> a owl:Class ;
    rdfs:label "Instrument"@en ;
    rdfs:comment "A tool or implement, especially one for precision work."@en ;
    rdfs:subClassOf <http://schema.org/Product> .

ns4:Organization a owl:Class ;
    rdfs:label "organization"@en ;
    rdfs:comment "An organization of some kind, e.g. research organization or business organization"@en ;
    ns4:example "Univerity Library in Leipzig, Museums of City Cologne" .

ns1:BFO_0000023 a owl:Class ;
    rdfs:label "role"@en ;
    ns1:BFO_0000179 "role" ;
    ns1:BFO_0000180 "Role" ;
    ns1:IAO_0000112 "John’s role of husband to Mary is dependent on Mary’s role of wife to John, and both are dependent on the object aggregate comprising John and Mary as member parts joined together through the relational quality of being married."@en,
        "the priest role"@en,
        "the role of a boundary to demarcate two neighboring administrative territories"@en,
        "the role of a building in serving as a military target"@en,
        "the role of a stone in marking a property boundary"@en,
        "the role of subject in a clinical trial"@en,
        "the student role"@en ;
    ns1:IAO_0000116 "BFO 2 Reference: One major family of examples of non-rigid universals involves roles, and ontologies developed for corresponding administrative purposes may consist entirely of representatives of entities of this sort. Thus ‘professor’, defined as follows,b instance_of professor at t =Def. there is some c, c instance_of professor role & c inheres_in b at t.denotes a non-rigid universal and so also do ‘nurse’, ‘student’, ‘colonel’, ‘taxpayer’, and so forth. (These terms are all, in the jargon of philosophy, phase sortals.) By using role terms in definitions, we can create a BFO conformant treatment of such entities drawing on the fact that, while an instance of professor may be simultaneously an instance of trade union member, no instance of the type professor role is also (at any time) an instance of the type trade union member role (any more than any instance of the type color is at any time an instance of the type length). If an ontology of employment positions should be defined in terms of roles following the above pattern, this enables the ontology to do justice to the fact that individuals instantiate the corresponding universals –  professor, sergeant, nurse – only during certain phases in their lives."@en ;
    ns1:IAO_0000600 "b is a role means: b is a realizable entity & b exists because there is some single bearer that is in some special physical, social, or institutional set of circumstances in which this bearer does not have to be& b is not such that, if it ceases to exist, then the physical make-up of the bearer is thereby changed. (axiom label in BFO2 Reference: [061-001])"@en ;
    ns1:IAO_0000602 "(forall (x) (if (Role x) (RealizableEntity x))) // axiom label in BFO2 CLIF: [061-001] " ;
    rdfs:isDefinedBy ns1:bfo.owl .

<http://schema.org/Product> a owl:Class .

<https://w3id.org/scholarlydata/ontology/conference-ontology.owl#OrganisedEvent> a owl:Class ;
    rdfs:label "Organised event"@en ;
    rdfs:comment "Any kind of organised event having a start and an end date."@en .

owl:Thing a owl:Class ;
    rdfs:label "Thing" .

ns2:Organization a owl:Class ;
    rdfs:label "organization"@en ;
    ns2:example "Universit\\u00e4tsbibliothek Leipzig, S\\u00e4chsisches Wirtschaftsarchiv, Museen der Stadt K\\u00f6ln" ;
    rdfs:comment "An organisation of some kind, e.g. research organisation or business organisation"@en ;
    owl:equivalentClass <http://schema.org/Organization> .

ns2:Person a owl:Class ;
    rdfs:label "person"@en ;
    ns2:example "Harald Sack, Tabea Tietz, Sasha Bruns, Etienne Posthumus" ;
    rdfs:comment "A resource that represents a single person."@en ;
    owl:equivalentClass <http://schema.org/Person> .

<http://www.ebi.ac.uk/swo/SWO_0000001> a owl:Class ;
    rdfs:label "software" ;
    ns1:IAO_0000115 "Computer software, or generally just software, is any set of machine-readable instructions (most often in the form of a computer program) that conform to a given syntax (sometimes referred to as a language) that is interpretable by a given processor and that directs a computer's processor to perform specific operations." ;
    ns1:IAO_0000119 "James Malone",
        "Modified in parts from https://en.wikipedia.org/wiki/Software",
        "Robert Stevens" ;
    rdfs:comment "AL 7.9.22: There are some reasoning oddities associated with marking IAO and SWO software as equivalent; once these are sorted out, the equivalence statement will take the place of this current parent-child relationship." .

<http://www.ebi.ac.uk/swo/SWO_0000002> a owl:Class ;
    rdfs:label "software license",
        "licence"@en ;
    ns1:IAO_0000115 "A licence is a legal instrument (usually by way of contract law, with or without printed material) governing the use or redistribution of the resource containing the licence." ;
    ns1:IAO_0000119 "Modified from http://en.wikipedia.org/wiki/Software_license" ;
    dcterms:creator "James Malone" .

ns2:Resource a owl:Class ;
    rdfs:label "resource"@en ;
    rdfs:comment "The most generic kind of a resource and may be associated with any kind of creative work, e.g. datasets, books, movies, photographs; offered products and services, e.g. data portals, data curation, data digitization; and intangible things, e.g. subjects of creative works, topics of events, offers, a list of enumerations."@en .

